Require branches to be maximal paths

PossiblyInfiniteTrees/PossiblyInfiniteTree/InfiniteTree.lean
@@ -10,39 +10,56 @@ namespace InfiniteTreeSkeleton
 
   def children (tree : InfiniteTreeSkeleton α) (node : List Nat) : InfiniteList α := fun n => tree (n :: node)
 
-  def branches_through (tree : InfiniteTreeSkeleton α) (node : List Nat) : Set (InfiniteList α) := fun branch =>
-    ∃ nodes : InfiniteList Nat, (∀ n : Nat, branch n = tree (nodes.take n).reverse) ∧ (nodes.take node.length).reverse = node
+  def branch_addresses_through (node : List Nat) : Set (InfiniteList Nat) := fun nodes =>
+    (nodes.take node.length).reverse = node
+
+  def branch_for_address (tree : InfiniteTreeSkeleton α) (nodes : InfiniteList Nat) : InfiniteList α := fun n => tree (nodes.take n).reverse
+
+  def branches_through (tree : InfiniteTreeSkeleton α) (node : List Nat) : Set (InfiniteList α) :=
+    (branch_addresses_through node).map tree.branch_for_address
 
   def branches (tree : InfiniteTreeSkeleton α) : Set (InfiniteList α) := tree.branches_through []
 
+  theorem branch_addresses_through_eq_union_branch_addresses_through_successors (node : List Nat) : branch_addresses_through node = fun nodes => ∃ (i : Nat), nodes ∈ branch_addresses_through (i :: node) := by
+    unfold branch_addresses_through
+    apply Set.ext
+    simp only [List.length_cons, List.reverse_eq_cons_iff, Membership.mem]
+    intro nodes
+    constructor
+    . intro h
+      exists nodes node.length
+      unfold InfiniteList.take
+      rw [List.append_cancel_right_eq]
+      rw [← List.reverse_eq_iff]
+      exact h
+    . intro h
+      rcases h with ⟨i, h⟩
+      unfold InfiniteList.take at h
+      rw [← List.reverse_inj] at h
+      rw [List.reverse_append] at h
+      rw [List.reverse_append] at h
+      simp only [List.reverse_cons, List.reverse_nil, List.nil_append, List.cons_append, List.reverse_reverse] at h
+      rw [List.cons.injEq] at h
+      exact h.right
+
   theorem branches_through_eq_union_branches_through_successors (tree : InfiniteTreeSkeleton α) (node : List Nat) : tree.branches_through node = fun b => ∃ (i : Nat), b ∈ tree.branches_through (i :: node) := by
     unfold branches_through
+    rw [branch_addresses_through_eq_union_branch_addresses_through_successors]
+    unfold Set.map
     apply Set.ext
-    simp only [List.length_cons, List.reverse_eq_cons_iff]
     intro b
     constructor
-    . intro ⟨nodes, h⟩
-      exists nodes node.length
+    . intro ⟨nodes, h, b_eq⟩
+      rcases h with ⟨i, h⟩
+      exists i
       exists nodes
-      constructor
-      . exact h.left
-      . unfold InfiniteList.take
-        rw [List.append_cancel_right_eq]
-        rw [← List.reverse_eq_iff]
-        exact h.right
     . intro h
       rcases h with ⟨i, nodes, h⟩
       exists nodes
       constructor
-      . exact h.left
-      . have hr := h.right
-        unfold InfiniteList.take at hr
-        rw [← List.reverse_inj] at hr
-        rw [List.reverse_append] at hr
-        rw [List.reverse_append] at hr
-        simp only [List.reverse_cons, List.reverse_nil, List.nil_append, List.cons_append, List.reverse_reverse] at hr
-        rw [List.cons.injEq] at hr
-        exact hr.right
+      . exists i
+        exact h.left
+      . exact h.right
 
 end InfiniteTreeSkeleton
 
