PossiblyInfiniteTrees/PossiblyInfiniteTree/FiniteDegreeTree/KoenigsLemma.lean
@@ -6,216 +6,284 @@ import PossiblyInfiniteTrees.PossiblyInfiniteTree.FiniteDegreeTree.Basic
 namespace FiniteDegreeTree
 
   theorem branches_through_finite_of_get_eq_none (tree : FiniteDegreeTree α) (node : List Nat) : tree.get node = none -> (tree.branches_through node).finite := by
-
     intro is_none
-    let branch_for_node : PossiblyInfiniteList α := ⟨fun n => if n ≤ node.length then tree.get (node.drop (node.length - n)) else none, by
-      intro n not_none
-      cases Decidable.em (n ≤ node.length) with
-      | inr lt => simp [lt] at not_none
-      | inl le =>
-        simp [le] at not_none
-        intro m
-        have m_le : m ≤ node.length := by apply Nat.le_trans; apply Nat.le_of_lt m.isLt; exact le
-        simp [m_le]
-        have no_orphans := tree.tree.no_orphans (node.drop (node.length - n)) not_none ⟨(node.drop (node.length - m)), by
-          exists (node.drop (node.length - n)).take (n - m)
-          rw [List.take_drop]
-          have : node.length - n + (n - m.val) = node.length - m.val := by
-            rw [← Nat.add_sub_assoc (by apply Nat.le_of_lt; exact m.isLt)]
-            rw [← Nat.sub_add_comm le]
-            simp
-          rw [this]
-          rw [← List.drop_append_of_le_length (by rw [List.length_take_of_le (by simp), Nat.sub_le_sub_iff_left m_le]; apply Nat.le_of_lt; exact m.isLt)]
-          simp
-        ⟩
-        exact no_orphans
-    ⟩
-    exists [branch_for_node]
-    constructor
-    . simp
-    . intro e
+    let nodes : InfiniteList Nat := fun n => if _isLt : n < node.length then node[node.length - (n+1)] else 0
+    let branch_for_node := tree.tree.branch_for_address nodes
+    have nodes_eq : ∀ n, n ≤ node.length -> (nodes.take n).reverse = node.drop (node.length - n) := by
+      intro n
+      induction n with
+      | zero => simp [InfiniteList.take]
+      | succ n ih =>
+        intro le
+        unfold InfiniteList.take
+        simp
+        rw [ih (by apply Nat.le_of_succ_le le)]
+        unfold nodes
+        have lt : n < node.length := by apply Nat.lt_of_succ_le le
+        simp [lt]
+        conv => right; rw [List.drop_eq_getElem_cons (by apply Nat.sub_lt_self; simp; exact le)]
+        have : node.length - (n + 1) + 1 = node.length - n := by omega
+        rw [this]
+    -- TODO: I think this could be decidable
+    cases Classical.em (tree.tree.branch_address_is_maximal nodes) with
+    | inl is_maximal =>
+      exists [branch_for_node]
       constructor
-      . intro h
-        simp at h
-        rw [h]
-        let nodes : InfiniteList Nat := fun n => if lt : n < node.length then node[node.length - (n+1)] else (tree.children node).length
-        have : ∀ n, n ≤ node.length -> (nodes.take n).reverse = node.drop (node.length - n) := by
-          intro n
-          induction n with
-          | zero => simp [InfiniteList.take]
-          | succ n ih =>
-            intro le
-            unfold InfiniteList.take
-            simp
-            rw [ih (by apply Nat.le_of_succ_le le)]
-            unfold nodes
-            have lt : n < node.length := by apply Nat.lt_of_succ_le le
-            simp [lt]
-            conv => right; rw [List.drop_eq_getElem_cons (by apply Nat.sub_lt_self; simp; exact le)]
-            have : node.length - (n + 1) + 1 = node.length - n := by omega
-            rw [this]
-        exists nodes
+      . simp
+      . intro e
         constructor
-        . intro n
+        . intro h
+          simp at h
+          rw [h]
+          exists nodes
+          constructor
+          . constructor
+            . unfold InfiniteTreeSkeleton.branch_addresses_through
+              simp only [Membership.mem]
+              rw [nodes_eq node.length]
+              . simp
+              . simp
+            . exact is_maximal
+          . rfl
+        . intro h
+          rcases h with ⟨nodes2, h⟩
+          rw [List.mem_singleton]
+          rw [PossiblyInfiniteList.eq_iff_same_on_all_indices]
+          intro n
+          rw [h.right]
+          unfold branch_for_node
+          simp only [PossiblyInfiniteTree.branch_for_address, InfiniteTreeSkeleton.branch_for_address]
           cases Decidable.em (n ≤ node.length) with
           | inl le =>
-            rw [this n le]
-            simp only [branch_for_node, le]
-            rfl
+            have : (nodes2.take n).reverse = node.drop (node.length - n) := by
+              conv => right; right; rw [← h.left.left]
+              rw [List.drop_reverse]
+              rw [InfiniteList.length_take]
+              rw [InfiniteList.take_after_take]
+              rw [Nat.sub_sub_self le]
+              simp [Nat.min_eq_right le]
+            rw [this, nodes_eq]
+            exact le
           | inr lt =>
-            simp only [branch_for_node, lt]
-            have no_orphans := tree.tree.no_orphans (nodes.take n).reverse
-            apply Eq.symm
-            apply Option.decidableEqNone.byContradiction
-            intro contra
-            specialize no_orphans contra ⟨node, by
-              exists ((nodes.skip (node.length)).take (n - node.length)).reverse
-              have : node = (nodes.take (node.length)).reverse := by
-                rw [this node.length]
-                . simp
-                . simp
-              conv => left; right; rw [this]
-              rw [← List.reverse_append]
-              rw [InfiniteList.combine_skip_take nodes n ⟨node.length, by apply Nat.lt_of_not_le; exact lt⟩]
-            ⟩
-            apply no_orphans
-            exact is_none
-        . rw [this]
-          . simp
-          . simp
-      . intro h
-        rcases h with ⟨nodes, h⟩
-        simp
-        rw [PossiblyInfiniteList.eq_iff_same_on_all_indices]
-        intro n
-        rw [h.left]
-        unfold branch_for_node
-        simp
-        cases Decidable.em (n ≤ node.length) with
-        | inl le =>
-          simp [le]
-          have : (nodes.take n).reverse = node.drop (node.length - n) := by
-            conv => right; right; rw [← h.right]
+            have nodes2_eq_none : tree.tree.infinite_tree (nodes2.take n).reverse = none := by
+              apply Option.decidableEqNone.byContradiction
+              intro contra
+              have no_orphans := tree.tree.no_orphans (nodes2.take n).reverse contra ⟨node, by
+                exists ((nodes2.skip (node.length)).take (n - node.length)).reverse
+                conv => left; right; rw [← h.left.left]
+                rw [← List.reverse_append]
+                rw [InfiniteList.combine_skip_take nodes2 n ⟨node.length, by apply Nat.lt_of_not_le; exact lt⟩]⟩
+              apply no_orphans
+              exact is_none
+            have nodes_eq_none : tree.tree.infinite_tree (nodes.take n).reverse = none := by
+              apply Option.decidableEqNone.byContradiction
+              intro contra
+              have no_orphans := tree.tree.no_orphans (nodes.take n).reverse contra ⟨node, by
+                exists ((nodes.skip (node.length)).take (n - node.length)).reverse
+                have : node = (nodes.take node.length).reverse := by
+                  rw [nodes_eq]
+                  . simp
+                  . simp
+                conv => left; right; rw [this]
+                rw [← List.reverse_append]
+                rw [InfiniteList.combine_skip_take nodes n ⟨node.length, by apply Nat.lt_of_not_le; exact lt⟩]⟩
+              apply no_orphans
+              exact is_none
+            rw [nodes2_eq_none, nodes_eq_none]
+    | inr not_maximal =>
+      exists []
+      constructor
+      . simp
+      . simp only [List.not_mem_nil, false_iff]
+        intro pil contra
+        rcases contra with ⟨nodes2, contra⟩
+        apply not_maximal
+
+        have nodes_eq_nodes2 : ∀ n, n ≤ node.length -> (nodes.take n).reverse = (nodes2.take n).reverse := by
+          intro n le
+          have : (nodes2.take n).reverse = node.drop (node.length - n) := by
+            conv => right; right; rw [← contra.left.left]
             rw [List.drop_reverse]
             rw [InfiniteList.length_take]
             rw [InfiniteList.take_after_take]
             rw [Nat.sub_sub_self le]
             simp [Nat.min_eq_right le]
           rw [this]
-          rfl
-        | inr lt =>
-          simp [lt]
+          rw [nodes_eq]
+          exact le
 
-          have no_orphans := tree.tree.no_orphans (nodes.take n).reverse
-          apply Option.decidableEqNone.byContradiction
-          intro contra
-          specialize no_orphans contra ⟨node, by
-            exists ((nodes.skip (node.length)).take (n - node.length)).reverse
-            conv => left; right; rw [← h.right]
-            rw [← List.reverse_append]
-            rw [InfiniteList.combine_skip_take nodes n ⟨node.length, by apply Nat.lt_of_not_le; exact lt⟩]
-          ⟩
-          apply no_orphans
-          exact is_none
+        intro n h
+        cases Decidable.em (n < node.length) with
+        | inl lt =>
+          rw [nodes_eq_nodes2]
+          apply contra.left.right
+          rw [← nodes_eq_nodes2]
+          . exact h
+          . apply Nat.succ_le_of_lt
+            exact lt
+          . apply Nat.le_of_lt
+            exact lt
+        | inr le =>
+          simp only [Nat.not_lt] at le
+          have : (nodes.take (n+1)).reverse = 0 :: (nodes.take n).reverse := by
+            conv => left; unfold nodes; simp only [InfiniteList.take]
+            rw [List.reverse_append, List.reverse_cons, List.reverse_nil, List.nil_append, List.singleton_append, List.cons_eq_cons]
+            constructor
+            . have : ¬ n < node.length := by apply Nat.not_lt_of_le; exact le
+              simp [this]
+            . rfl
+          rw [← this]
+          exact h
+
+  theorem branches_through_finite_of_children_empty (tree : FiniteDegreeTree α) (node : List Nat) : tree.children node = [] -> (tree.branches_through node).finite := by
+    intro h
+    cases Option.decidableEqNone.em (tree.get node = none) with
+    | inl eq_none => apply branches_through_finite_of_get_eq_none; exact eq_none
+    | inr neq_none =>
+      let nodes : InfiniteList Nat := fun n => if _isLt : n < node.length then node[node.length - (n+1)] else 0
+      let branch_for_node := tree.tree.branch_for_address nodes
+      have nodes_eq : ∀ n, n ≤ node.length -> (nodes.take n).reverse = node.drop (node.length - n) := by
+        intro n
+        induction n with
+        | zero => simp [InfiniteList.take]
+        | succ n ih =>
+          intro le
+          unfold InfiniteList.take
+          simp
+          rw [ih (by apply Nat.le_of_succ_le le)]
+          unfold nodes
+          have lt : n < node.length := by apply Nat.lt_of_succ_le le
+          simp [lt]
+          conv => right; rw [List.drop_eq_getElem_cons (by apply Nat.sub_lt_self; simp; exact le)]
+          have : node.length - (n + 1) + 1 = node.length - n := by omega
+          rw [this]
+      exists [branch_for_node]
+      constructor
+      . simp
+      . intro branch
+        simp only [List.mem_singleton]
+        constructor
+        . intro pre
+          rw [pre]
+          exists nodes
+          constructor
+          . constructor
+            . unfold InfiniteTreeSkeleton.branch_addresses_through; simp only [Membership.mem]; rw [nodes_eq node.length]; simp; simp
+            . intro n
+              cases Decidable.em (n < node.length) with
+              | inl lt =>
+                intro contra
+                apply False.elim
+                apply tree.tree.no_orphans node neq_none ⟨(nodes.take (n+1)).reverse, by
+                  exists ((nodes.skip (n+1)).take (node.length - (n+1))).reverse
+                  rw [← List.reverse_append]
+                  cases Decidable.em (n + 1 < node.length) with
+                  | inl lt2 =>
+                    rw [InfiniteList.combine_skip_take nodes node.length ⟨n+1, lt2⟩]
+                    rw [nodes_eq]
+                    . simp
+                    . simp
+                  | inr le2 =>
+                    have : n+1 = node.length := by
+                      apply Nat.eq_of_lt_succ_of_not_lt
+                      . apply Nat.succ_lt_succ; exact lt
+                      . exact le2
+                    rw [this]
+                    simp only [Nat.sub_self, InfiniteList.take, List.append_nil]
+                    rw [nodes_eq]
+                    . simp
+                    . simp⟩
+                exact contra
+              | inr le =>
+                intro eq_none
+                unfold InfiniteList.take at eq_none
+                rw [List.reverse_append, List.reverse_cons, List.reverse_nil, List.nil_append, List.singleton_append] at eq_none
+                unfold nodes at eq_none
+                simp only [le, ↓reduceDIte] at eq_none
+                exact eq_none
+          . rfl
+        . intro pre
+          rcases pre with ⟨nodes2, pre⟩
+          rw [pre.right]
+          rw [PossiblyInfiniteList.eq_iff_same_on_all_indices]
+          intro n
+          unfold branch_for_node
+          simp only [PossiblyInfiniteTree.branch_for_address, InfiniteTreeSkeleton.branch_for_address]
+          cases Decidable.em (n ≤ node.length) with
+          | inl le =>
+            have : (nodes2.take n).reverse = node.drop (node.length - n) := by
+              conv => right; right; rw [← pre.left.left]
+              rw [List.drop_reverse]
+              rw [InfiniteList.length_take]
+              rw [InfiniteList.take_after_take]
+              rw [Nat.sub_sub_self le]
+              simp [Nat.min_eq_right le]
+            rw [this, nodes_eq]
+            exact le
+          | inr lt =>
+            have nodes2_eq_none : tree.tree.infinite_tree (nodes2.take n).reverse = none := by
+              apply Option.decidableEqNone.byContradiction
+              intro contra
+              have no_orphans := tree.tree.no_orphans (nodes2.take n).reverse contra ⟨(nodes2.take (node.length + 1)).reverse, by
+                exists ((nodes2.skip (node.length + 1)).take (n - (node.length + 1))).reverse
+                rw [← List.reverse_append]
+                cases Decidable.em (node.length + 1 < n) with
+                | inl lt2 => rw [InfiniteList.combine_skip_take nodes2 n ⟨node.length+1, lt2⟩]
+                | inr le2 =>
+                  have : node.length + 1 = n := by
+                    apply Nat.eq_of_lt_succ_of_not_lt
+                    . apply Nat.succ_lt_succ; apply Nat.lt_of_not_le; exact lt
+                    . exact le2
+                  rw [this]
+                  simp only [Nat.sub_self, InfiniteList.take, List.append_nil]⟩
+              apply no_orphans
+              have := tree.each_successor_none_of_children_empty node h (nodes2 node.length)
+              simp only [InfiniteList.take, List.reverse_append, List.reverse_cons, List.reverse_nil, List.nil_append, List.singleton_append]
+              rw [pre.left.left]
+              exact this
+            have nodes_eq_none : tree.tree.infinite_tree (nodes.take n).reverse = none := by
+              apply Option.decidableEqNone.byContradiction
+              intro contra
+              have no_orphans := tree.tree.no_orphans (nodes.take n).reverse contra ⟨(nodes.take (node.length + 1)).reverse, by
+                exists ((nodes.skip (node.length + 1)).take (n - (node.length + 1))).reverse
+                rw [← List.reverse_append]
+                cases Decidable.em (node.length + 1 < n) with
+                | inl lt2 => rw [InfiniteList.combine_skip_take nodes n ⟨node.length+1, lt2⟩]
+                | inr le2 =>
+                  have : node.length + 1 = n := by
+                    apply Nat.eq_of_lt_succ_of_not_lt
+                    . apply Nat.succ_lt_succ; apply Nat.lt_of_not_le; exact lt
+                    . exact le2
+                  rw [this]
+                  simp only [Nat.sub_self, InfiniteList.take, List.append_nil]⟩
+              apply no_orphans
+              have := tree.each_successor_none_of_children_empty node h (nodes node.length)
+              simp only [InfiniteList.take, List.reverse_append, List.reverse_cons, List.reverse_nil, List.nil_append, List.singleton_append]
+              rw [nodes_eq]
+              . simp only [Nat.sub_self, List.drop_zero]
+                exact this
+              . simp
+            rw [nodes2_eq_none, nodes_eq_none]
 
   theorem branches_through_finite_of_each_successor_branches_through_finite (tree : FiniteDegreeTree α) (node : List Nat) : (∀ i, (tree.branches_through (i :: node)).finite) -> (tree.branches_through node).finite := by
 
     intro h
     have dec := Classical.typeDecidableEq (PossiblyInfiniteList α)
-    let branch_for_node : PossiblyInfiniteList α := ⟨fun n => if n ≤ node.length then tree.get (node.drop (node.length - n)) else none, by
-      intro n not_none
-      cases Decidable.em (n ≤ node.length) with
-      | inr lt => simp [lt] at not_none
-      | inl le =>
-        simp [le] at not_none
-        intro m
-        have m_le : m ≤ node.length := by apply Nat.le_trans; apply Nat.le_of_lt m.isLt; exact le
-        simp [m_le]
-        have no_orphans := tree.tree.no_orphans (node.drop (node.length - n)) not_none ⟨(node.drop (node.length - m)), by
-          exists (node.drop (node.length - n)).take (n - m)
-          rw [List.take_drop]
-          have : node.length - n + (n - m.val) = node.length - m.val := by
-            rw [← Nat.add_sub_assoc (by apply Nat.le_of_lt; exact m.isLt)]
-            rw [← Nat.sub_add_comm le]
-            simp
-          rw [this]
-          rw [← List.drop_append_of_le_length (by rw [List.length_take_of_le (by simp), Nat.sub_le_sub_iff_left m_le]; apply Nat.le_of_lt; exact m.isLt)]
-          simp
-        ⟩
-        exact no_orphans
-    ⟩
-    let branches_for_i (i : Nat) := Classical.choose (h i)
-    let target_list : List (PossiblyInfiniteList α) := (branch_for_node :: ((tree.children node).zipIdx_with_lt.map (fun (_, i) => branches_for_i i.val)).flatten).eraseDupsKeepRight
-    exists target_list
-    constructor
-    . apply List.nodup_eraseDupsKeepRight
-    . intro branch
-      unfold target_list
-      rw [List.mem_eraseDupsKeepRight]
-      simp
+
+    cases Option.decidableEqNone.em ((tree.get (0::node)) = none) with
+    | inl childs_empty => apply branches_through_finite_of_children_empty; apply tree.children_empty_of_first_successor_none; exact childs_empty
+    | inr childs_not_empty =>
+      let branches_for_i (i : Nat) := Classical.choose (h i)
+      let target_list : List (PossiblyInfiniteList α) := ((tree.children node).zipIdx_with_lt.map (fun (_, i) => branches_for_i i.val)).flatten.eraseDupsKeepRight
+      exists target_list
       constructor
-      . intro pre
-        cases pre with
-        | inl eq =>
-          let nodes : InfiniteList Nat := fun n => if lt : n < node.length then node[node.length - (n+1)] else (tree.children node).length
-          have : ∀ n, n ≤ node.length -> (nodes.take n).reverse = node.drop (node.length - n) := by
-            intro n
-            induction n with
-            | zero => simp [InfiniteList.take]
-            | succ n ih =>
-              intro le
-              unfold InfiniteList.take
-              simp
-              rw [ih (by apply Nat.le_of_succ_le le)]
-              unfold nodes
-              have lt : n < node.length := by apply Nat.lt_of_succ_le le
-              simp [lt]
-              conv => right; rw [List.drop_eq_getElem_cons (by apply Nat.sub_lt_self; simp; exact le)]
-              have : node.length - (n + 1) + 1 = node.length - n := by omega
-              rw [this]
-          exists nodes
-          constructor
-          . rw [eq]
-            intro n
-            cases Decidable.em (n ≤ node.length) with
-            | inl le =>
-              rw [this n le]
-              simp only [branch_for_node, le]
-              rfl
-            | inr lt =>
-              simp only [branch_for_node, lt]
-              have : tree.tree.infinite_tree (nodes.take (node.length + 1)).reverse = none := by
-                have child_none : (tree.children node)[nodes node.length]? = none := by
-                  apply List.getElem?_eq_none
-                  unfold nodes
-                  simp
-                rw [getElem_children_eq_getElem_lifted_children, PossiblyInfiniteTree.getElem_children_eq_get] at child_none
-                unfold PossiblyInfiniteTree.get at child_none
-                unfold InfiniteList.take
-                simp
-                rw [this]
-                . simp
-                  exact child_none
-                . simp
-              have le : node.length + 1 ≤ n := by apply Nat.succ_le_of_lt; apply Nat.lt_of_not_ge; exact lt
-              cases Nat.eq_or_lt_of_le le with
-              | inl eq => simp [← eq, this]
-              | inr lt =>
-                have no_orphans := tree.tree.no_orphans (nodes.take n).reverse
-                apply Eq.symm
-                apply Option.decidableEqNone.byContradiction
-                intro contra
-                specialize no_orphans contra ⟨(nodes.take (node.length + 1)).reverse, by
-                  exists ((nodes.skip (node.length + 1)).take (n - (node.length + 1))).reverse
-                  rw [← List.reverse_append]
-                  rw [InfiniteList.combine_skip_take nodes n ⟨node.length + 1, lt⟩]
-                ⟩
-                apply no_orphans
-                exact this
-          . rw [this]
-            . simp
-            . simp
-        | inr pre =>
+      . apply List.nodup_eraseDupsKeepRight
+      . intro branch
+        unfold target_list
+        rw [List.mem_eraseDupsKeepRight]
+        simp only [List.mem_flatten, List.mem_map, Prod.exists]
+        constructor
+        . intro pre
           rcases pre with ⟨branches, ex_i, branch_mem⟩
           rcases ex_i with ⟨_, i, _, eq⟩
           rw [branches_through_eq_union_branches_through_successors]
@@ -225,76 +293,46 @@ namespace FiniteDegreeTree
           unfold branches_for_i at eq
           rw [eq]
           exact branch_mem
-      . intro pre
-        rw [branches_through_eq_union_branches_through_successors] at pre
-        rcases pre with ⟨i, pre⟩
-        cases Decidable.em (i < (tree.children node).length) with
-        | inl lt =>
-          apply Or.inr
-          exists branches_for_i i
-          constructor
-          . let i_fin : Fin (tree.children node).length := ⟨i, lt⟩
-            exists (tree.children node)[i]
-            exists i_fin
+        . intro pre
+          rw [branches_through_eq_union_branches_through_successors] at pre
+          rcases pre with ⟨i, pre⟩
+          cases Decidable.em (i < (tree.children node).length) with
+          | inl lt =>
+            exists branches_for_i i
             constructor
-            . rw [List.mem_zipIdx_with_lt_iff_mem_zipIdx]
-              rw [List.mem_zipIdx_iff_getElem?]
-              simp [i_fin]
-            . rfl
-          . have spec := Classical.choose_spec (h i)
-            unfold branches_for_i
-            rw [spec.right]
-            exact pre
-        | inr not_lt =>
-          apply Or.inl
-          rcases pre with ⟨nodes, pre⟩
-          unfold branch_for_node
-          rw [PossiblyInfiniteList.eq_iff_same_on_all_indices]
-          intro n
-          rw [pre.left n]
-          have pre_r := pre.right
-          simp [InfiniteList.take] at pre_r
-          simp
-          cases Decidable.em (n ≤ node.length) with
-          | inl le =>
-            simp [le]
-            have : (nodes.take n).reverse = node.drop (node.length - n) := by
-              conv => right; right; rw [← pre_r.right]
-              rw [List.drop_reverse]
-              rw [InfiniteList.length_take]
-              rw [InfiniteList.take_after_take]
-              rw [Nat.sub_sub_self le]
-              simp [Nat.min_eq_right le]
-            rw [this]
-            rfl
-          | inr lt =>
-            simp [lt]
-            have : tree.tree.infinite_tree (nodes.take (node.length + 1)).reverse = none := by
-              have : (tree.children node)[nodes node.length]? = none := by
-                apply List.getElem?_eq_none
-                rw [pre_r.left]
-                apply Nat.le_of_not_gt
-                exact not_lt
-              rw [getElem_children_eq_getElem_lifted_children, PossiblyInfiniteTree.getElem_children_eq_get] at this
-              unfold PossiblyInfiniteTree.get at this
-              unfold InfiniteList.take
-              simp
-              rw [pre_r.right]
-              exact this
-            have le : node.length + 1 ≤ n := by apply Nat.succ_le_of_lt; apply Nat.lt_of_not_ge; exact lt
-            cases Nat.eq_or_lt_of_le le with
-            | inl eq => rw [← eq]; exact this
-            | inr lt =>
-              have no_orphans := tree.tree.no_orphans (nodes.take n).reverse
-              apply Option.decidableEqNone.byContradiction
-              intro contra
-              specialize no_orphans contra ⟨(nodes.take (node.length + 1)).reverse, by
-                exists ((nodes.skip (node.length + 1)).take (n - (node.length + 1))).reverse
-                rw [← List.reverse_append]
-                rw [InfiniteList.combine_skip_take nodes n ⟨node.length + 1, lt⟩]
-              ⟩
-              apply no_orphans
-              exact this
+            . let i_fin : Fin (tree.children node).length := ⟨i, lt⟩
+              exists (tree.children node)[i]
+              exists i_fin
+              constructor
+              . rw [List.mem_zipIdx_with_lt_iff_mem_zipIdx]
+                rw [List.mem_zipIdx_iff_getElem?]
+                simp [i_fin]
+              . rfl
+            . have spec := Classical.choose_spec (h i)
+              unfold branches_for_i
+              rw [spec.right]
+              exact pre
+          | inr not_lt =>
+            rcases pre with ⟨nodes, pre⟩
+            apply False.elim
+            apply childs_not_empty
+            have node_eq := pre.left.left
+            unfold InfiniteTreeSkeleton.branch_addresses_through at node_eq
+            simp only [List.length_cons, InfiniteList.take, List.reverse_append, List.reverse_cons, List.reverse_nil, List.nil_append, List.singleton_append, Membership.mem] at node_eq
+            rw [List.cons_eq_cons] at node_eq
+            rw [← node_eq.right]
+            apply pre.left.right
+            have : (tree.children node)[nodes node.length]? = none := by
+              apply List.getElem?_eq_none
+              rw [node_eq.left]
+              apply Nat.le_of_not_gt
+              exact not_lt
+            rw [getElem_children_eq_getElem_lifted_children, PossiblyInfiniteTree.getElem_children_eq_get] at this
+            unfold PossiblyInfiniteTree.get at this
+            unfold InfiniteList.take
+            rw [List.reverse_append, List.reverse_cons, List.reverse_nil, List.nil_append, List.singleton_append]
+            rw [node_eq.right]
+            exact this
 
   noncomputable def infinite_branching_node_for_depth_of_branches_infinite (tree : FiniteDegreeTree α) (not_finite : ¬ tree.branches.finite) : (depth : Nat) -> { node : List Nat // node.length = depth ∧ ¬ (tree.branches_through node).finite }
   | .zero => ⟨[], by constructor; rfl; exact not_finite⟩
@@ -360,8 +398,13 @@ namespace FiniteDegreeTree
     specialize h branch (by
       exists nodes
       constructor
-      . intro n
-        rfl
+      . constructor
+        . rfl
+        . intro n contra
+          apply False.elim
+          apply all_infinite (n+1)
+          apply branches_through_finite_of_get_eq_none
+          exact contra
       . rfl
     )
 
